More progress on ExternValidity.dfy

Test/dafny0/ExternValidity.dfy
@@ -6,7 +6,10 @@ module ExternalInvariants {
     predicate Valid() 
       reads this, Repr 
       ensures Valid() ==> this in Repr
-
+    static predicate AllValid(vs: set<Validatable>) {
+      && (forall v :: v in vs ==> v.Valid())
+      && (forall v, v' :: (v in vs && v' in vs && v != v') ==> v.Repr !! v'.Repr)
+    }
   }
 
   class NotAtomic extends Validatable {
@@ -19,7 +22,9 @@ module ExternalInvariants {
       this.y := 2*x;
       this.Repr := {this};
     }
-
+    constructor NotValid() {
+    }
+    
     predicate Valid() 
       reads this, Repr 
       ensures Valid() ==> this in Repr
@@ -28,16 +33,85 @@ module ExternalInvariants {
       && this in Repr
     }
 
-    method Update(newX: int) 
+    method Update(x: int) 
+      requires Validatable.AllValid(set v: Validatable | true)
+      modifies this
+      ensures Validatable.AllValid(set v: Validatable | true)
+    {
+      assert this in set v: Validatable | v.Valid();
+      this.x := x;
+      this.y := 2*x;
+    }
+  }
+
+  trait {:extern} ExternalNotAtomic {
+    method Update(x: int) 
+      requires Validatable.AllValid(set v: Validatable | true)
+      modifies this
+      ensures Validatable.AllValid(set v: Validatable | true)
+  }
+
+  method {:extern} MakeExternalNotAtomic() returns (res: ExternalNotAtomic)
+    requires Validatable.AllValid(set v: Validatable | true)
+    ensures Validatable.AllValid(set v: Validatable | true)
+  {
+    var internal := new NotAtomic(73);
+    res := new AsExternalNotAtomic(internal);
+  }
+
+  method {:extern} MakeExternalNotAtomic_NotValid() returns (res: ExternalNotAtomic)
+    requires Validatable.AllValid(set v: Validatable | true)
+    ensures Validatable.AllValid(set v: Validatable | true)
+  {
+    res := new AsExternalNotAtomic.NotValid();
+  }
+
+  class AsExternalNotAtomic extends ExternalNotAtomic, Validatable {
+    const wrapped: NotAtomic
+    predicate Valid() 
+      reads this, Repr 
+      ensures Valid() ==> this in Repr
+    {
+      this in Repr && wrapped.Valid()
+    }
+    constructor(wrapped: NotAtomic) ensures Valid() {
+      this.wrapped := wrapped;
+      this.Repr := {this, wrapped} + wrapped.Repr;
+    }
+    constructor NotValid() {
+    }
+    method Update(x: int) 
+      requires Validatable.AllValid(set v: Validatable | true)
+      modifies this
+      ensures Validatable.AllValid(set v: Validatable | true)
+    {
+      wrapped.Update(x);
+    }
+  }
+
+  class Rational extends Validatable {
+
+    var a: int
+    var b: int
+
+    predicate Valid() 
+      reads this, Repr 
+      ensures Valid() ==> this in Repr
+    {
+      && 0 <= a
+      && 0 < b
+      && this in Repr
+    }
+
+    method Invert() 
       requires Valid()
-      requires forall v: Validatable :: v.Valid()
+      requires a != 0
       modifies this
       ensures Valid()
     {
-      this.x := newX;
-      this.y := 2*x;
-
-      assert forall v: Validatable :: v.Valid();
+      var tmp := a;
+      a := b;
+      b := tmp;
     }
   }
 }
